RelationalCalculus/Eq.lean
@@ -2,16 +2,48 @@ import RelationalCalculus.Basic
 import RelationalCalculus.Order
 open Relation
 
-
+namespace Relation
 -- Define custom equality for Relation based on union order (inclusion)
-def Relation.eq (R S : Relation α β) : Prop :=
+def eq (R S : Relation α β) : Prop :=
   R ≤ S ∧ S ≤ R
 
 -- Notation for extensional equality
-infix:50 " ≃ " => Relation.eq
+infix:50 " ≃ " => eq
 
+-- *** Equivalence Properties ***
+-- Reflexivity
+@[refl]
+theorem eq_refl (R : Relation α β) : R ≃ R :=
+  ⟨le_refl R, le_refl R⟩
 
-theorem Relation.eval_eq_iff_eq {R S : Relation α β} : (eval R = eval S) ↔ (R ≃ S) := by
+-- Symmetry
+@[symm]
+theorem eq_symm {R S : Relation α β} (h : R ≃ S) : S ≃ R :=
+  ⟨h.2, h.1⟩
+
+-- Transitivity
+@[trans]
+theorem eq_trans {R S T : Relation α β} (h₁ : R ≃ S) (h₂ : S ≃ T) : R ≃ T :=
+  ⟨le_trans h₁.1 h₂.1, le_trans h₂.2 h₁.2⟩
+end Relation
+
+-- Create Setoid instance
+-- A Setoid is a set together with an equivalence relation
+instance : Setoid (Relation α β) where
+  r :=  Relation.eq
+  iseqv := {
+    refl := Relation.eq_refl
+    symm := Relation.eq_symm
+    trans := Relation.eq_trans
+  }
+
+instance : HasEquiv (Relation α β) where
+Equiv := Relation.eq
+
+namespace Relation
+-- *** Theorems Relating Order Equivalence to Evaluation Equality ***
+-- Our equivalence relation defined in terms of ordering actually implies equivalence in terms of evaluation. This is because we defined ordering in terms of evaluation (see Order.lean).
+theorem eval_eq_iff_eq {R S : Relation α β} : (eval R = eval S) ↔ (R ≃ S) := by
   constructor
   · intro h
     unfold eq
@@ -33,25 +65,8 @@ theorem Relation.eval_eq_iff_eq {R S : Relation α β} : (eval R = eval S) ↔ (
     · exact (le_rel_iff_le_eval.mp h.left) a b
     · exact (le_rel_iff_le_eval.mp h.right) a b
 
-
-
-
--- Prove reflexivity
-@[refl]
-theorem Relation.eq_refl (R : Relation α β) : R ≃ R :=
-  ⟨le_refl R, le_refl R⟩
-
--- Prove symmetry
-@[symm]
-theorem Relation.eq_symm {R S : Relation α β} (h : R ≃ S) : S ≃ R :=
-  ⟨h.2, h.1⟩
-
--- Prove transitivity
-@[trans]
-theorem Relation.eq_trans {R S T : Relation α β} (h₁ : R ≃ S) (h₂ : S ≃ T) : R ≃ T :=
-  ⟨le_trans h₁.1 h₂.1, le_trans h₂.2 h₁.2⟩
-
-theorem Relation.eq_iff_eval_eq {R S : Relation α β} :
+-- TODO: This theorem is very similar to eval_eq_iff_eq, do we need both of them?
+theorem eq_iff_eval_eq {R S : Relation α β} :
     R ≃ S ↔ (∀ a b, eval R a b ↔ eval S a b) := by
   constructor
   · intro h
@@ -64,14 +79,15 @@ theorem Relation.eq_iff_eval_eq {R S : Relation α β} :
     · intro a b hs
       exact (h a b).2 hs
 
--- Extentional equality implies evaluation equality
 
-theorem Relation.eq_to_eval {R S : Relation α β} (h : R ≃ S) :
+
+-- Extentional equality implies evaluation equality
+theorem eq_to_eval {R S : Relation α β} (h : R ≃ S) :
     eval R = eval S := by
   funext a b
   exact propext (Relation.eq_iff_eval_eq.1 h a b)
 
-theorem Relation.eval_to_eq {R S : Relation α β} (h: eval R = eval S) : R ≃ S := by
+theorem eval_to_eq {R S : Relation α β} (h: eval R = eval S) : R ≃ S := by
   unfold eq
   constructor
   · intro a b hR
@@ -81,18 +97,7 @@ theorem Relation.eval_to_eq {R S : Relation α β} (h: eval R = eval S) : R ≃ 
     rw [h]
     exact hS
 
--- Create Setoid instance
--- A Setoid is a set together with an equivalence relation
-instance : Setoid (Relation α β) where
-  r :=  Relation.eq
-  iseqv := {
-    refl := Relation.eq_refl
-    symm := Relation.eq_symm
-    trans := Relation.eq_trans
-  }
-
-instance : HasEquiv (Relation α β) where
-Equiv := Relation.eq
+end Relation
 
 def Relation.Setoid := @instSetoidRelation
 def Relation.HasEquiv := @instHasEquivRelation
