RelationalCalculus/Order.lean
@@ -8,8 +8,9 @@ open Relation
  instance : LE (Relation α β) where
     le R S := ∀ a b, eval R a b → eval S a b
 
+namespace Relation
 --  R ≤  S if and only if they eval to pair functions that are less than or equal to eachother.
-theorem Relation.le_rel_iff_le_eval {α β : Type u} {R S : Relation α β} :
+theorem le_rel_iff_le_eval {α β : Type u} {R S : Relation α β} :
   R ≤ S ↔ (eval R ≤ eval S) := by
   constructor
   · intro h
@@ -21,16 +22,21 @@ theorem Relation.le_rel_iff_le_eval {α β : Type u} {R S : Relation α β} :
 
 
 -- Prove that this ordering is reflexive
-theorem Relation.le_refl (R : Relation α β) : R ≤ R := by
+theorem le_refl (R : Relation α β) : R ≤ R := by
   intros _ _ h
   exact h
 
 -- Prove that this ordering is transitive
-theorem Relation.le_trans {R S T : Relation α β} (h₁ : R ≤ S) (h₂ : S ≤ T) : R ≤ T := by
+theorem le_trans {R S T : Relation α β} (h₁ : R ≤ S) (h₂ : S ≤ T) : R ≤ T := by
   intros a b hR
   exact h₂ a b (h₁ a b hR)
 
+end Relation
+
 -- Create the Preorder instance
+-- This automatically enables us to use ≤ notation to indicate ordering of relations. Note that the use of ≤ is essentially a semantic operation since it is defined in terms of evaluation. Later we'll see that linear implication (⊸) give as an equivalent algebraic definition of subrelations with the relation R ⊸ S corresponding to the semantics S ≤ R.
+-- Since turning R ⊸ S into a statement about ording requires defining propositions as relations, we get to this in Logic.lean.
+
 instance : Preorder (Relation α β) where
   le := (· ≤ ·)
   le_refl := Relation.le_refl
